deps/poulet4/lib/ValueUtil.v
@@ -1,7 +1,7 @@
 Require Import Coq.Strings.String Coq.ZArith.ZArith Coq.Lists.List.
 Require Import Poulet4.Value Poulet4.Typed Poulet4.P4String
                Poulet4.SyntaxUtil Poulet4.AList Poulet4.Sublist.
-Require Import Poulet4.P4Notations.
+Require Import Poulet4.P4Notations Poulet4.Monads.Monad Poulet4.Monads.Option.
 Import ListNotations.
 
 Section ValueUtil.
@@ -215,68 +215,68 @@ Section ValueUtil.
     | ValBaseSenumField t e v => ValBaseSenumField t e (eval_val_to_sval v)
     end.
 
-  Definition uninit_sval_of_typ (hvalid : option bool) (typ : @P4Type tags_t): option Sval :=
-    let fix uninit_sval_of_typ' hvalid (typ : @P4Type tags_t) : option Sval :=
-      match typ with
-      | TypBool => Some (ValBaseBool None)
-      | TypInt w => Some (ValBaseInt (Zrepeat None (Z.of_N w)))
-      | TypBit w => Some (ValBaseBit (Zrepeat None (Z.of_N w)))
-      | TypArray typ size =>
-          match uninit_sval_of_typ' hvalid typ with
-          | Some sv => Some (ValBaseStack (Zrepeat sv (Z.of_N size)) 0)
-          | None => None
-          end
-      | TypTuple typs
-      | TypList typs => 
-          match lift_option (List.map (uninit_sval_of_typ' hvalid) typs) with
-          | Some svs => Some (ValBaseTuple svs)
-          | None => None
-          end
-      | TypRecord fields =>
-          match lift_option_kv (kv_map (uninit_sval_of_typ' hvalid) fields) with
-          | Some kvs => Some (ValBaseRecord (P4String.clear_AList_tags kvs))
-          | None => None
-          end
-      | TypHeader fields =>
-          match lift_option_kv (kv_map (uninit_sval_of_typ' hvalid) fields) with
-          | Some kvs => Some (ValBaseHeader (P4String.clear_AList_tags kvs) hvalid)
-          | None => None
-          end
-      | TypHeaderUnion fields =>
-          match lift_option_kv (kv_map (uninit_sval_of_typ' hvalid) fields) with
-          | Some kvs => Some (ValBaseUnion (P4String.clear_AList_tags kvs))
-          | None => None
-          end
-      | TypStruct fields =>
-          match lift_option_kv (kv_map (uninit_sval_of_typ' hvalid) fields) with
-          | Some kvs => Some (ValBaseStruct (P4String.clear_AList_tags kvs))
-          | None => None
-          end
-      | TypNewType _ typ' => uninit_sval_of_typ' hvalid typ'
-      (* TypTypeName should have been already resolved *)
-      | TypTypeName _ => None
-      (* Two possibilities for senum:
-        1. Use the default values (similar to the enum type):
-            For enum values with an underlying type the default value is 0. (7.3.)
-        2. Use the underlying types's uninitialized values:
-            Since an senum's underlying type is either bit or int, it can also be uninitialized
-            by the underlying types.
-        The current implementation follows the option 2. *)
-      | TypEnum tname (Some typ') members => uninit_sval_of_typ' hvalid typ'
-      (* The P4Spec does not specify the unintialized values for the following types,
-        so we use the default values for now. (7.3.) 
-        Note that this design choice makes the svals output from uninit_sval_of_typ different
-        from uninit_sval_of_sval and val_to_sval. *)
-      | TypVarBit w => Some (ValBaseVarbit w [])
-      | TypInteger => Some (ValBaseInteger 0)
-      | TypError => Some (ValBaseError "NoError")
-      | TypEnum tname None members => 
-          (* Empty members is a syntax error *)
-          if (Nat.eqb (List.length members) 0) then None
-          else Some (ValBaseEnumField (str tname) (str (List.hd !"" members)))
-      | _ => None
-      end
-    in uninit_sval_of_typ' hvalid typ.
+  Fixpoint uninit_sval_of_typ
+           (hvalid : option bool) (typ : @P4Type tags_t): option Sval :=
+    match typ with
+    | TypBool => Some (ValBaseBool None)
+    | TypInt w => Some (ValBaseInt (Zrepeat None (Z.of_N w)))
+    | TypBit w => Some (ValBaseBit (Zrepeat None (Z.of_N w)))
+    | TypArray typ size =>
+      let^ sv := uninit_sval_of_typ hvalid typ in
+      ValBaseStack (Zrepeat sv (Z.of_N size)) 0
+    | TypTuple typs
+    | TypList typs => 
+      sequence (List.map (uninit_sval_of_typ hvalid) typs) >>| ValBaseTuple
+    | TypRecord fields =>
+      sequence
+        (List.map
+           (fun '({| P4String.str := x |}, t) =>
+              uninit_sval_of_typ hvalid t >>| pair x)
+           fields) >>| ValBaseRecord
+    | TypHeader fields =>
+      let^ kvs :=
+         sequence
+           (List.map
+              (fun '({| P4String.str := x |}, t) =>
+                 uninit_sval_of_typ hvalid t >>| pair x)
+              fields) in
+      ValBaseHeader kvs hvalid
+    | TypHeaderUnion fields =>
+      sequence
+        (List.map
+           (fun '({| P4String.str := x |}, t) =>
+              uninit_sval_of_typ hvalid t >>| pair x)
+           fields) >>| ValBaseUnion
+    | TypStruct fields =>
+      sequence
+        (List.map
+           (fun '({| P4String.str := x |}, t) =>
+              uninit_sval_of_typ hvalid t >>| pair x)
+           fields) >>| ValBaseStruct
+    | TypNewType _ typ' => uninit_sval_of_typ hvalid typ'
+    (* TypTypeName should have been already resolved *)
+    | TypTypeName _ => None
+    (* Two possibilities for senum:
+       1. Use the default values (similar to the enum type):
+       For enum values with an underlying type the default value is 0. (7.3.)
+       2. Use the underlying types's uninitialized values:
+       Since an senum's underlying type is either bit or int, it can also be uninitialized
+       by the underlying types.
+       The current implementation follows the option 2. *)
+    | TypEnum tname (Some typ') members => uninit_sval_of_typ hvalid typ'
+    (* The P4Spec does not specify the unintialized values for the following types,
+       so we use the default values for now. (7.3.) 
+       Note that this design choice makes the svals output from uninit_sval_of_typ different
+       from uninit_sval_of_sval and val_to_sval. *)
+    | TypVarBit w => Some (ValBaseVarbit w [])
+    | TypInteger => Some (ValBaseInteger 0)
+    | TypError => Some (ValBaseError "NoError")
+    | TypEnum tname None members => 
+      (* Empty members is a syntax error *)
+      if (Nat.eqb (List.length members) 0) then None
+      else Some (ValBaseEnumField (str tname) (str (List.hd !"" members)))
+    | _ => None
+    end.
   (* Type without uninitialized svals:
       TypString: can be used only for compile-time constant string values (7.1.),
                   one cannot declare variables with a string type (7.1.5.),
